proof/correctness/Correctness_Wots.ec
@@ -8,6 +8,109 @@ require import XMSS_IMPL XMSS_IMPL_PP Generic.
 
 require import Array2 Array3 Array8 Array32 Array67 Array2144.
 
+print mkseq.
+
+op w32Array_to_intlist (x : W32.t Array67.t) = mkseq (fun (i : int) => to_uint x.[i]) 67.
+
+lemma wots_checksum_correctness (msg : W32.t Array67.t) :
+    len1 = XMSS_WOTS_LEN1 /\ w = XMSS_WOTS_W =>
+    equiv [Mp(Syscall).__csum ~ WOTS.checksum :
+      arg{1} = msg /\ arg{2} = w32Array_to_intlist msg /\ 
+      forall (k : int), 0 <= k < 67 => 0 <= to_uint msg.[k] <= (w - 1) ==> 
+        to_uint res{1} = to_uint res{2}].
+proof.
+rewrite /XMSS_WOTS_LEN1 /XMSS_WOTS_W ; move => [len1_val w_val].
+proc => /=.
+while (
+  #pre /\
+  i{2} = to_uint i{1} /\ 0 <= to_uint i{1} <= 64 /\
+  m{2} = w32Array_to_intlist msg_base_w{1} /\
+  0 <= i{2} <= len1 /\
+  to_uint csum{1} = checksum{2} /\
+  0 <= to_uint csum{1} <= W32.max_uint
+).
+- auto => />. move => &1 H0 H1 H2 H3 H4 H5 H6 H7 ; do split; 1,2,3,7: by rewrite to_uintD /#.
+    + smt().
+    + smt().
+    + rewrite w_val !to_uintD /=. admit.
+    + move => ?. rewrite to_uintD. admit.
+    + rewrite len1_val ultE of_uintK to_uintD /= /#.
+    + rewrite len1_val ultE to_uintD /= /#.
+- auto => />. move => * ; do split; 1,2: by rewrite len1_val. auto => /> *. rewrite of_uintK /#. 
+qed.
+
+op w32Array_to_intlist_3 (x : W32.t Array3.t) = mkseq (fun (i : int) => to_uint x.[i]) 3.
+
+lemma base_w_correct (o : W32.t Array3.t, _in : W8.t Array2.t) : 
+    floor (log2 w%r) = XMSS_WOTS_LOG_W => 
+    equiv[M(Syscall).__base_w_3_2 ~ BaseW.base_w : 
+      arg{1}=(o, _in) /\ arg{2}=(to_list _in, 3) ==> res{2} = w32Array_to_intlist_3 res{1}].
+proof.
+rewrite /XMSS_WOTS_LOG_W ; move => logw_val.
+proc.
+wp ; sp.
+while (
+  X{2} = to_list input{1} /\
+  outlen{2} = 3 /\
+  0 <= to_uint i{1} <= 3 /\ consumed{2} = to_uint i{1} /\ out{2} = to_uint i{1} /\
+  0 <= to_uint bits{1} <= 16 /\ (* bits <= 8 * inlen = 8 * 2 = 16 *)
+  bits{2} = to_uint bits{1} /\
+  to_uint total{1} = to_uint total{2} /\
+  forall (k : int), 0 <= k < to_uint i{1} => to_uint output{1}.[k] = nth witness base_w{2} k
+).
+- if.
+    + move => &1 &2 H0. move : H0 => [#] H0 H1 H2 H3 H4 H5 H6 H7 H8 H9 H10 H11 H12. split ; smt(@W64). 
+    + auto => /> &1 &2 H0 H1 H2 H3 H4 H5 ; do split.
+        * rewrite to_uintD /#.
+        * rewrite to_uintD /#.
+        * rewrite to_uintD /#. 
+        * rewrite to_uintD /#.
+        * by rewrite logw_val.
+        * admit.
+        * admit.
+        * rewrite ultE of_uintK to_uintD /#.
+        * rewrite ultE of_uintK to_uintD /#.
+    + auto => />. move => &1 &2 H0 H1 H2 H3 H4 H5 H6 H7 H8 ; do split.
+        * rewrite to_uintD /#.
+        * rewrite to_uintD /#.
+        * rewrite to_uintD /#. 
+        * rewrite to_uintD /#.
+        * rewrite to_uintD /#.
+        * admit.
+        * rewrite logw_val. admit.
+        * admit. 
+        * move => k k_ge0 ?. admit.
+        * rewrite ultE of_uintK to_uintD /#.
+        * rewrite ultE of_uintK to_uintD /#.
+- skip => />. progress. smt. rewrite /w32Array_to_intlist_3. admit.
+
+
+
+
+
+
+
+
+
+
+
+
+
+
+
+
+
+
+lemma base_w_post : hoare [BaseW.base_w : 0 < outlen ==> all (fun (k : int) => 0 <= k < w) res].
+proof.
+proc.
+while (
+  #pre /\
+  0 <= consumed <= outlen /\
+  0 <= out <= outlen /\ out = consumed /\
+  0 <= bits <= 8 * outlen
+).
+
 lemma nosmt shr_ge0 (input : W8.t Array32.t) (i : W64.t) :
     0 <= to_uint i < 32 =>
     0 <= to_uint ((SHR_32 (zeroextu32 input.[to_uint i]) (truncateu8 ((of_int 4))%W64)).`6 `&` (of_int 15)%W32).
