proof/correctness/Correctness_Mem.ec
@@ -8,7 +8,7 @@ require import Array128 Array4.
 require import XMSS_IMPL.
 
 require import Array128 Array4.
-require import XMSS_IMPL.
+require import XMSS_IMPL XMSS_IMPL_PP.
 
 lemma memset_4_post (input : W8.t Array4.t, v : W8.t) :
     hoare [M(Syscall).__memset_u8_4 : arg=(input, v) ==> 
@@ -44,16 +44,48 @@ while (
 - progress ; [ smt(@W64) | smt ].
 qed.
 
-lemma memset_4_ll : islossless M(Syscall).__memset_u8_4.
+lemma memset_zero_post (x : W8.t Array4.t) :
+    hoare [Mp(Syscall).__memset_zero_u8 : true ==> forall (k : int), 0 <= k < 4 => (res.[k] = W8.zero)].
 proof.
 proc.
-while (0 <= to_uint i <= 4) (4 - (to_uint i)) ; auto => /> * ; last by smt(@W64).
-do split; 1,3: by rewrite to_uintD_small /#. smt(@W64).
+while (
+  0 <= to_uint i <= 4 /\ 
+  (forall (k : int), 0 <= k < to_uint i => (a.[k] = W8.zero))
+); auto => /> *.
+- do split.
+  + smt(@W64).
+  + smt(@W64).
+  + move => ???. rewrite get_setE ; smt(@W64).
+- progress ; [ smt(@W64) | smt ].
 qed.
 
-lemma memset_128_ll : islossless M(Syscall).__memset_u8_128.
+lemma load_store mem (ptr : W64.t) (v : W8.t) :
+    loadW8 (storeW8 mem (to_uint ptr) v) (to_uint ptr) = v 
+      by rewrite /storeW8 /loadW8 get_setE ifT.
+
+lemma memset_ptr_post (ptr : W64.t, len : W64.t, v : W8.t) :
+    hoare [Mp(Syscall).__memset_u8_ptr : 
+      0 <= to_uint len < W64.max_uint /\ 
+      0 <= to_uint ptr + to_uint len < W64.max_uint /\
+      0 <= to_uint ptr < W64.max_uint /\
+      arg=(ptr, len, v) ==>
+        forall (k:int), 0 <= k < to_uint len => (loadW8 Glob.mem (W64.to_uint (ptr  + (W64.of_int k)))) = v].
 proof.
 proc.
-while (0 <= to_uint i <= 128) (128 - (to_uint i)) ; auto => /> * ; last by smt(@W64).
-do split; 1,3: by rewrite to_uintD_small /#. smt(@W64).
+while (
+  #pre /\
+  (to_uint ptr) <= to_uint _ptr <= (to_uint (ptr + inlen)) /\
+  0 <= to_uint i <= to_uint inlen /\
+  (forall (k:int), 0 <= k < to_uint i => ((loadW8 Glob.mem (W64.to_uint (_ptr  + (W64.of_int k)))) = value))
+).
+- auto => /> * ; do split.
+    + rewrite to_uintD_small ; smt(@W64).
+    + move => ?. rewrite !to_uintD //=. admit.
+    + smt(@W64).
+    + smt(@W64).
+    + move => *. rewrite /storeW8 /loadW8 get_setE ifT //. congr. admit.
+- auto ; progress.
+    + rewrite to_uintD_small //= ; smt(@W64).
+    + smt.
+    + admit.
 qed.
